Fix everything

common.v
@@ -2,7 +2,6 @@ From WR Require Import imports.
 
 Definition context := list tm.
 
-
 Inductive lookup : nat -> context -> tm -> Prop :=
   | here : forall {A Γ}, lookup 0 (A :: Γ) (A ⟨shift⟩)
   | there : forall {n A Γ B},
@@ -12,56 +11,3 @@ Definition lookup_good_renaming ξ Γ Δ :=
   forall i A, lookup i Γ A -> lookup (ξ i) Δ A⟨ξ⟩.
 
 Derive Inversion lookup_inv with (forall i Γ A, lookup i Γ A).
-
-(*
-Fixpoint dep_ith Γ i :=
-  match Γ , i with
-  | (A :: Γ), 0 => ren_tm shift A
-  | (A :: Γ), (S i) => ren_tm shift (dep_ith Γ i)
-  | _, _ => tVoid
-  end.
-
-Notation ith Γ i := (nth i Γ tVoid).
-
-Lemma dep_ith_ren_tm (Γ : context) (A : tm) (x : fin) :
-  dep_ith (A :: Γ) (S x) = ren_tm shift (dep_ith Γ x).
-Proof. done. Qed.
-
-Definition good_renaming ξ Γ Δ :=
-  forall i, i ∈ dom Γ -> ξ i ∈ dom Δ /\ dep_ith Δ (ξ i) = ren_tm ξ (dep_ith Γ i).
-
-Lemma dep_ith_shift Γ i :
-  dep_ith Γ i = ren_tm (Nat.add (S i)) (ith Γ i).
-Proof.
-  elim : Γ i.
-  - hauto q:on.
-  - move => A Γ h.
-    case => [|i].
-    + done.
-    + simpl.
-      rewrite h.
-      by asimpl.
-Qed.
-
-Lemma ith_skipn n i (Γ : context) :
-  ith (skipn n Γ) i = ith Γ (n + i).
-  move : n i.
-  elim : Γ.
-  - hauto lq:on inv:nat.
-  - move => A Γ ih n i.
-    case : i; qauto l:on inv:nat.
-Qed.
-
-Lemma good_renaming_truncate n Γ :
-  good_renaming (Nat.add n) (skipn n Γ) Γ .
-Proof.
-  rewrite /good_renaming => i h /=.
-  repeat rewrite dep_ith_shift.
-  rewrite ith_skipn.
-  split.
-  - rewrite skipn_length in h.
-    lia.
-  - asimpl. f_equal.
-    fext => ?; asimpl; lia.
-Qed.
-*)
